refactor(library): minor reorg

library/data/bitvec.lean
@@ -9,7 +9,7 @@ This is a work-in-progress, and contains additions to other theories.
 -/
 import data.tuple
 
-definition bitvec (n : ℕ) := tuple bool n
+def bitvec (n : ℕ) := tuple bool n
 
 namespace bitvec
 
@@ -17,15 +17,15 @@ open nat
 open tuple
 
 -- Create a zero bitvector
-definition zero { n : ℕ } : bitvec n := tuple.repeat ff
+def zero {n : ℕ} : bitvec n := tuple.repeat ff
 
 -- Create a bitvector with the constant one.
-definition one {n : ℕ} : bitvec (succ n) := tuple.append (tuple.repeat ff : bitvec n) [ tt ]
+def one {n : ℕ} : bitvec (succ n) := tuple.append (tuple.repeat ff : bitvec n) [ tt ]
 
 section shift
 
   -- shift left
-  definition shl {n:ℕ} : bitvec n → ℕ → bitvec n
+  def shl {n : ℕ} : bitvec n → ℕ → bitvec n
     | x i :=
        if le : i ≤ n then
          let eq := nat.sub_add_cancel le in
@@ -34,7 +34,7 @@ section shift
          zero
 
   -- unsigned shift right
-  definition ushr {n:ℕ} : bitvec n → ℕ → bitvec n
+  def ushr {n : ℕ} : bitvec n → ℕ → bitvec n
     | x i :=
       if le : i ≤ n then
         let y : bitvec (n-i) := @firstn _ _ _ (sub_le n i) x in
@@ -45,7 +45,7 @@ section shift
         zero
 
   -- signed shift right
-  definition sshr {m:ℕ} : bitvec (succ m) → ℕ → bitvec (succ m)
+  def sshr {m : ℕ} : bitvec (succ m) → ℕ → bitvec (succ m)
     | x i :=
       let n := succ m in
       if le : i ≤ n then
@@ -60,48 +60,47 @@ section shift
 end shift
 
 section bitwise
-  variable { n : ℕ }
+  variable {n : ℕ}
 
-  definition not : bitvec n → bitvec n := map bnot
-  definition and : bitvec n → bitvec n → bitvec n := map₂ band
-  definition or  : bitvec n → bitvec n → bitvec n := map₂ bor
-  definition xor : bitvec n → bitvec n → bitvec n := map₂ bxor
+  def not : bitvec n → bitvec n := map bnot
+  def and : bitvec n → bitvec n → bitvec n := map₂ band
+  def or  : bitvec n → bitvec n → bitvec n := map₂ bor
+  def xor : bitvec n → bitvec n → bitvec n := map₂ bxor
 
 end bitwise
 
 section arith
+  variable {n : ℕ}
 
-  variable { n : ℕ }
-
-  protected definition xor3 (x:bool) (y:bool) (c:bool) := bxor (bxor x y) c
-  protected definition carry (x:bool) (y:bool) (c:bool) :=
+  protected def xor3 (x:bool) (y:bool) (c:bool) := bxor (bxor x y) c
+  protected def carry (x:bool) (y:bool) (c:bool) :=
     x && y || x && c || y && c
 
-  definition neg : bitvec n → bitvec n
+  def neg : bitvec n → bitvec n
   | x :=
     let f := λy c, (y || c, bxor y c) in
     prod.snd (map_accumr f x ff)
 
   -- Add with carry (no overflow)
-  definition adc : bitvec n → bitvec n → bool → bitvec (n+1)
+  def adc : bitvec n → bitvec n → bool → bitvec (n+1)
   | x y c :=
     let f := λx y c, (bitvec.carry x y c, bitvec.xor3 x y c) in
     let z := tuple.map_accumr₂ f x y c in
     prod.fst z :: prod.snd z
 
-  definition add : bitvec n → bitvec n → bitvec n
+  def add : bitvec n → bitvec n → bitvec n
   | x y := tail (adc x y ff)
 
-  protected definition borrow (x:bool) (y:bool) (b:bool) :=
+  protected def borrow (x:bool) (y:bool) (b:bool) :=
     bnot x && y || bnot x && b || y && b
 
   -- Subtract with borrow
-  definition sbb : bitvec n → bitvec n → bool → bool × bitvec n
+  def sbb : bitvec n → bitvec n → bool → bool × bitvec n
   | x y b :=
     let f := λx y c, (bitvec.borrow x y c, bitvec.xor3 x y c) in
     tuple.map_accumr₂ f x y b
 
-  definition sub : bitvec n → bitvec n → bitvec n
+  def sub : bitvec n → bitvec n → bitvec n
   | x y := prod.snd (sbb x y ff)
 
   instance : has_zero (bitvec n) := has_zero.mk zero
@@ -110,7 +109,7 @@ section arith
   instance : has_sub (bitvec n)  := has_sub.mk  sub
   instance : has_neg (bitvec n)  := has_neg.mk  neg
 
-  definition mul : bitvec n → bitvec n → bitvec n
+  def mul : bitvec n → bitvec n → bitvec n
   | x y :=
     let f := λr b, cond b (r + r + y) (r + r) in
     list.foldl f 0 (to_list x)
@@ -121,26 +120,26 @@ end arith
 section comparison
   variable {n : ℕ}
 
-  definition uborrow : bitvec n → bitvec n → bool := λx y, prod.fst (sbb x y ff)
+  def uborrow : bitvec n → bitvec n → bool := λx y, prod.fst (sbb x y ff)
 
-  definition ult (x y : bitvec n) : Prop := uborrow x y = tt
-  definition ugt (x y : bitvec n) : Prop := ult y x
+  def ult (x y : bitvec n) : Prop := uborrow x y = tt
+  def ugt (x y : bitvec n) : Prop := ult y x
 
-  definition ule (x y : bitvec n) : Prop := ¬ (ult y x)
-  definition uge : bitvec n → bitvec n → Prop := λx y, ule y x
+  def ule (x y : bitvec n) : Prop := ¬ (ult y x)
+  def uge : bitvec n → bitvec n → Prop := λx y, ule y x
 
-  definition sborrow : bitvec (succ n) → bitvec (succ n) → bool := λx y,
+  def sborrow : bitvec (succ n) → bitvec (succ n) → bool := λx y,
      bool.cases_on
        (head x)
        (bool.cases_on (head y) (uborrow (tail x) (tail y)) tt)
        (bool.cases_on (head y) ff (uborrow (tail x) (tail y)))
 
-  definition slt : bitvec (succ n) → bitvec (succ n) → Prop := λx y,
+  def slt : bitvec (succ n) → bitvec (succ n) → Prop := λx y,
      sborrow x y = tt
 
-  definition sgt : bitvec (succ n) → bitvec (succ n) → Prop := λx y, slt y x
-  definition sle : bitvec (succ n) → bitvec (succ n) → Prop := λx y, ¬ (slt y x)
-  definition sge : bitvec (succ n) → bitvec (succ n) → Prop := λx y, sle y x
+  def sgt : bitvec (succ n) → bitvec (succ n) → Prop := λx y, slt y x
+  def sle : bitvec (succ n) → bitvec (succ n) → Prop := λx y, ¬ (slt y x)
+  def sge : bitvec (succ n) → bitvec (succ n) → Prop := λx y, sle y x
 
 end comparison
 
@@ -148,10 +147,9 @@ section from_bitvec
   variable {α : Type}
 
   -- Convert a bitvector to another number.
-  definition from_bitvec [p : has_add α] [q0 : has_zero α] [q1 : has_one α] {n:nat} (v:bitvec n) : α :=
-    let f : α → bool → α := λr b, cond b (r + r + 1) (r + r) in
-    list.foldl f (0 : α) (to_list v)
+  def from_bitvec [has_add α] [has_zero α] [has_one α] {n : nat} (v : bitvec n) : α :=
+  let f : α → bool → α := λr b, cond b (r + r + 1) (r + r) in
+  list.foldl f (0 : α) (to_list v)
 end from_bitvec
-
 
 end bitvec
