library/init/nat.lean
@@ -10,77 +10,6 @@ import init.order
 notation `ℕ` := nat
 
 namespace nat
-  protected lemma zero_add : ∀ n : ℕ, 0 + n = n
-  | 0     := rfl
-  | (n+1) := congr_arg succ (zero_add n)
-
-  lemma succ_add : ∀ n m : ℕ, (succ n) + m = succ (n + m)
-  | n 0     := rfl
-  | n (m+1) := congr_arg succ (succ_add n m)
-
-  protected lemma add_comm : ∀ n m : ℕ, n + m = m + n
-  | n 0     := eq.symm (nat.zero_add n)
-  | n (m+1) :=
-    suffices succ (n + m) = succ (m + n), from
-      eq.symm (succ_add m n) ▸ this,
-    congr_arg succ (add_comm n m)
-
-  protected lemma bit0_succ_eq (n : ℕ) : bit0 (succ n) = succ (succ (bit0 n)) :=
-  show succ (succ n + n) = succ (succ (n + n)), from
-  congr_arg succ (succ_add n n)
-
-  protected lemma bit1_eq_succ_bit0 (n : ℕ) : bit1 n = succ (bit0 n) :=
-  rfl
-
-  protected lemma bit1_succ_eq (n : ℕ) : bit1 (succ n) = succ (succ (bit1 n)) :=
-  eq.trans (nat.bit1_eq_succ_bit0 (succ n)) (congr_arg succ (nat.bit0_succ_eq n))
-
-  lemma succ_ne_zero (n : ℕ) : succ n ≠ 0 :=
-  assume h, nat.no_confusion h
-
-  lemma succ_ne_self : ∀ n : ℕ, succ n ≠ n
-  | 0     h := absurd h (nat.succ_ne_zero 0)
-  | (n+1) h := succ_ne_self n (nat.no_confusion h (λ h, h))
-
-  protected lemma one_ne_zero : 1 ≠ (0 : ℕ) :=
-  assume h, nat.no_confusion h
-
-  protected lemma bit0_ne_zero : ∀ n : ℕ, n ≠ 0 → bit0 n ≠ 0
-  | 0     h := absurd rfl h
-  | (n+1) h := nat.succ_ne_zero _
-
-  protected lemma bit1_ne_zero (n : ℕ) : bit1 n ≠ 0 :=
-  show succ (n + n) ≠ 0, from
-  succ_ne_zero (n + n)
-
-  protected lemma bit1_ne_one : ∀ n : ℕ, n ≠ 0 → bit1 n ≠ 1
-  | 0     h h1 := absurd rfl h
-  | (n+1) h h1 := nat.no_confusion h1 (λ h2, absurd h2 (nat.succ_ne_zero _))
-
-  protected lemma bit0_ne_one : ∀ n : ℕ, bit0 n ≠ 1
-  | 0     h := absurd h (ne.symm nat.one_ne_zero)
-  | (n+1) h :=
-    have h1 : succ (succ (n + n)) = 1, from succ_add n n ▸ h,
-    nat.no_confusion h1
-      (λ h2, absurd h2 (succ_ne_zero (n + n)))
-
-  protected lemma add_self_ne_one : ∀ (n : ℕ), n + n ≠ 1
-  | 0     h := nat.no_confusion h
-  | (n+1) h :=
-    have h1 : succ (succ (n + n)) = 1, from succ_add n n ▸ h,
-    nat.no_confusion h1 (λ h2, absurd h2 (nat.succ_ne_zero (n + n)))
-
-  protected lemma bit1_ne_bit0 : ∀ (n m : ℕ), bit1 n ≠ bit0 m
-  | 0     m     h := absurd h (ne.symm (nat.add_self_ne_one m))
-  | (n+1) 0     h :=
-    have h1 : succ (bit0 (succ n)) = 0, from h,
-    absurd h1 (nat.succ_ne_zero _)
-  | (n+1) (m+1) h :=
-    have h1 : succ (succ (bit1 n)) = succ (succ (bit0 m)), from
-      nat.bit0_succ_eq m ▸ nat.bit1_succ_eq n ▸ h,
-    have h2 : bit1 n = bit0 m, from
-      nat.no_confusion h1 (λ h2', nat.no_confusion h2' (λ h2'', h2'')),
-    absurd h2 (bit1_ne_bit0 n m)
 
   inductive le (a : ℕ) : ℕ → Prop
   | nat_refl : le a    -- use nat_refl to avoid overloading le.refl
@@ -88,10 +17,6 @@ namespace nat
 
   instance : has_le ℕ :=
   ⟨nat.le⟩
-
-  attribute [refl]
-  protected def le_refl : ∀ a : ℕ, a ≤ a :=
-  le.nat_refl
 
   @[reducible] protected def lt (n m : ℕ) := succ n ≤ m
 
@@ -126,148 +51,41 @@ namespace nat
       | is_false xney := is_false (λ h, nat.no_confusion h (λ xeqy, absurd xeqy xney))
       end
 
+  def {u} repeat {α : Type u} (f : ℕ → α → α) : ℕ → α → α
+  | 0         a := a
+  | (succ n)  a := f n (repeat n a)
+
+  instance : inhabited ℕ :=
+  ⟨nat.zero⟩
+
   /- properties of inequality -/
 
-  protected lemma le_of_eq {n m : ℕ} (p : n = m) : n ≤ m :=
-  p ▸ le.nat_refl n
+  @[refl] protected def le_refl : ∀ a : ℕ, a ≤ a :=
+  le.nat_refl
 
   lemma le_succ (n : ℕ) : n ≤ succ n :=
   le.step (nat.le_refl n)
 
-  lemma pred_le : ∀ (n : ℕ), pred n ≤ n
-  | 0        := le.nat_refl 0
-  | (succ a) := le.step (le.nat_refl a)
-
-  attribute [simp]
-  lemma le_succ_iff_true (n : ℕ) : n ≤ succ n ↔ true :=
-  iff_true_intro (le_succ n)
-
-  attribute [simp]
-  lemma pred_le_iff_true (n : ℕ) : pred n ≤ n ↔ true :=
-  iff_true_intro (pred_le n)
-
-  protected lemma le_trans {n m k : ℕ} (h1 : n ≤ m) : m ≤ k → n ≤ k :=
-  le.rec h1 (λ p h2, le.step)
-
-  lemma le_succ_of_le {n m : ℕ} (h : n ≤ m) : n ≤ succ m :=
-  nat.le_trans h (le_succ m)
-
-  lemma le_of_succ_le {n m : ℕ} (h : succ n ≤ m) : n ≤ m :=
-  nat.le_trans (le_succ n) h
-
-  protected lemma le_of_lt {n m : ℕ} (h : n < m) : n ≤ m :=
-  le_of_succ_le h
-
   lemma succ_le_succ {n m : ℕ} : n ≤ m → succ n ≤ succ m :=
   λ h, le.rec (nat.le_refl (succ n)) (λ a b, le.step) h
+
+  lemma zero_le : ∀ (n : ℕ), 0 ≤ n
+  | 0     := nat.le_refl 0
+  | (n+1) := le.step (zero_le n)
+
+  lemma zero_lt_succ (n : ℕ) : 0 < succ n :=
+  succ_le_succ (zero_le n)
+
+  lemma not_succ_le_zero : ∀ (n : ℕ), succ n ≤ 0 → false
+  .
+
+  lemma not_lt_zero (a : ℕ) : ¬ a < 0 := not_succ_le_zero a
 
   lemma pred_le_pred {n m : ℕ} : n ≤ m → pred n ≤ pred m :=
   λ h, le.rec (nat.le_refl (pred n)) (λ n, nat.rec (λ a b, b) (λ a b c, le.step) n) h
 
   lemma le_of_succ_le_succ {n m : ℕ} : succ n ≤ succ m → n ≤ m :=
   pred_le_pred
-
-  lemma le_succ_of_pred_le {n m : ℕ} : pred n ≤ m → n ≤ succ m :=
-  nat.cases_on n le.step (λ a, succ_le_succ)
-
-  lemma not_succ_le_zero : ∀ (n : ℕ), succ n ≤ 0 → false
-  .
-
-  lemma succ_le_zero_iff_false (n : ℕ) : succ n ≤ 0 ↔ false :=
-  iff_false_intro (not_succ_le_zero n)
-
-  lemma not_succ_le_self : ∀ n : ℕ, ¬succ n ≤ n :=
-  λ n, nat.rec (not_succ_le_zero 0) (λ a b c, b (le_of_succ_le_succ c)) n
-
-  attribute [simp]
-  lemma succ_le_self_iff_false (n : ℕ) : succ n ≤ n ↔ false :=
-  iff_false_intro (not_succ_le_self n)
-
-  lemma zero_le : ∀ (n : ℕ), 0 ≤ n
-  | 0     := nat.le_refl 0
-  | (n+1) := le.step (zero_le n)
-
-  attribute [simp]
-  lemma zero_le_iff_true (n : ℕ) : 0 ≤ n ↔ true :=
-  iff_true_intro (zero_le n)
-
-  protected lemma one_le_bit1 (n : ℕ) : 1 ≤ bit1 n :=
-  show 1 ≤ succ (bit0 n), from
-  succ_le_succ (zero_le (bit0 n))
-
-  protected lemma one_le_bit0 : ∀ (n : ℕ), n ≠ 0 → 1 ≤ bit0 n
-  | 0     h := absurd rfl h
-  | (n+1) h :=
-    suffices 1 ≤ succ (succ (bit0 n)), from
-      eq.symm (nat.bit0_succ_eq n) ▸ this,
-    succ_le_succ (zero_le (succ (bit0 n)))
-
-  def lt.step {n m : ℕ} : n < m → n < succ m := le.step
-
-  lemma zero_lt_succ (n : ℕ) : 0 < succ n :=
-  succ_le_succ (zero_le n)
-
-  attribute [simp]
-  lemma zero_lt_succ_iff_true (n : ℕ) : 0 < succ n ↔ true :=
-  iff_true_intro (zero_lt_succ n)
-
-  protected lemma lt_trans {n m k : ℕ} (h₁ : n < m) : m < k → n < k :=
-  nat.le_trans (le.step h₁)
-
-  protected lemma lt_of_le_of_lt {n m k : ℕ} (h₁ : n ≤ m) : m < k → n < k :=
-  nat.le_trans (succ_le_succ h₁)
-
-  protected lemma lt_of_lt_of_le {n m k : ℕ} : n < m → m ≤ k → n < k := nat.le_trans
-
-  protected lemma lt_irrefl (n : ℕ) : ¬n < n :=
-  not_succ_le_self n
-
-  lemma lt_self_iff_false (n : ℕ) : n < n ↔ false :=
-  iff_false_intro (λ h, absurd h (nat.lt_irrefl n))
-
-  lemma self_lt_succ (n : ℕ) : n < succ n := nat.le_refl (succ n)
-
-  attribute [simp]
-  lemma self_lt_succ_iff_true (n : ℕ) : n < succ n ↔ true :=
-  iff_true_intro (self_lt_succ n)
-
-  def lt.base (n : ℕ) : n < succ n := nat.le_refl (succ n)
-
-  lemma le_lt_antisymm {n m : ℕ} (h₁ : n ≤ m) (h₂ : m < n) : false :=
-  nat.lt_irrefl n (nat.lt_of_le_of_lt h₁ h₂)
-
-  protected lemma le_antisymm {n m : ℕ} (h₁ : n ≤ m) : m ≤ n → n = m :=
-  le.cases_on h₁ (λ a, rfl) (λ a b c, absurd (nat.lt_of_le_of_lt b c) (nat.lt_irrefl n))
-
-  instance : weak_order ℕ :=
-    ⟨ @nat.le, @nat.le_refl, @nat.le_trans, @nat.le_antisymm ⟩
-
-  lemma lt_le_antisymm {n m : ℕ} (h₁ : n < m) (h₂ : m ≤ n) : false :=
-  le_lt_antisymm h₂ h₁
-
-  protected lemma nat.lt_asymm {n m : ℕ} (h₁ : n < m) : ¬ m < n :=
-  le_lt_antisymm (nat.le_of_lt h₁)
-
-  lemma not_lt_zero (a : ℕ) : ¬ a < 0 := not_succ_le_zero a
-
-  attribute [simp]
-  lemma lt_zero_iff_false (a : ℕ) : a < 0 ↔ false :=
-  iff_false_intro (not_lt_zero a)
-
-  protected lemma eq_or_lt_of_le {a b : ℕ} (h : a ≤ b) : a = b ∨ a < b :=
-  le.cases_on h (or.inl rfl) (λ n h, or.inr (succ_le_succ h))
-
-  protected lemma le_of_eq_or_lt {a b : ℕ} (h : a = b ∨ a < b) : a ≤ b :=
-  or.elim h nat.le_of_eq nat.le_of_lt
-
-  lemma succ_lt_succ {a b : ℕ} : a < b → succ a < succ b :=
-  succ_le_succ
-
-  lemma lt_of_succ_lt {a b : ℕ} : succ a < b → a < b :=
-  le_of_succ_le
-
-  lemma lt_of_succ_lt_succ {a b : ℕ} : succ a < succ b → a < b :=
-  le_of_succ_le_succ
 
   instance decidable_le : ∀ a b : ℕ, decidable (a ≤ b)
   | 0     b     := is_true (zero_le b)
@@ -281,64 +99,32 @@ namespace nat
   instance decidable_lt : ∀ a b : ℕ, decidable (a < b) :=
   λ a b, nat.decidable_le (succ a) b
 
-  protected lemma lt_or_ge : ∀ (a b : ℕ), a < b ∨ a ≥ b
-  | a 0     := or.inr (zero_le a)
-  | a (b+1) :=
-    match lt_or_ge a b with
-    | or.inl h := or.inl (le_succ_of_le h)
-    | or.inr h :=
-      match nat.eq_or_lt_of_le h with
-      | or.inl h1 := or.inl (h1 ▸ self_lt_succ b)
-      | or.inr h1 := or.inr h1
-      end
-    end
-
-  protected def {u} lt_ge_by_cases {a b : ℕ} {C : Type u} (h₁ : a < b → C) (h₂ : a ≥ b → C) : C :=
-  decidable.by_cases h₁ (λ h, h₂ (or.elim (nat.lt_or_ge a b) (λ a, absurd a h) (λ a, a)))
-
-  protected def {u} lt_by_cases {a b : ℕ} {C : Type u} (h₁ : a < b → C) (h₂ : a = b → C)
-    (h₃ : b < a → C) : C :=
-  nat.lt_ge_by_cases h₁ (λ h₁,
-    nat.lt_ge_by_cases h₃ (λ h, h₂ (nat.le_antisymm h h₁)))
-
-  protected lemma lt_trichotomy (a b : ℕ) : a < b ∨ a = b ∨ b < a :=
-  nat.lt_by_cases (λ h, or.inl h) (λ h, or.inr (or.inl h)) (λ h, or.inr (or.inr h))
-
-  protected lemma eq_or_lt_of_not_lt {a b : ℕ} (hnlt : ¬ a < b) : a = b ∨ b < a :=
-  or.elim (nat.lt_trichotomy a b)
-    (λ hlt, absurd hlt hnlt)
-    (λ h, h)
+  protected lemma eq_or_lt_of_le {a b : ℕ} (h : a ≤ b) : a = b ∨ a < b :=
+  le.cases_on h (or.inl rfl) (λ n h, or.inr (succ_le_succ h))
 
   lemma lt_succ_of_le {a b : ℕ} : a ≤ b → a < succ b :=
   succ_le_succ
 
-  lemma lt_of_succ_le {a b : ℕ} (h : succ a ≤ b) : a < b := h
-
-  lemma succ_le_of_lt {a b : ℕ} (h : a < b) : succ a ≤ b := h
-
-  attribute [simp]
-  lemma succ_sub_succ_eq_sub (a b : ℕ) : succ a - succ b = a - b :=
+  @[simp] lemma succ_sub_succ_eq_sub (a b : ℕ) : succ a - succ b = a - b :=
   nat.rec_on b
     (show succ a - succ zero = a - zero, from (eq.refl (succ a - succ zero)))
     (λ b, congr_arg pred)
 
-  lemma sub_eq_succ_sub_succ (a b : ℕ) : a - b = succ a - succ b :=
-  eq.symm (succ_sub_succ_eq_sub a b)
+  lemma not_succ_le_self : ∀ n : ℕ, ¬succ n ≤ n :=
+  λ n, nat.rec (not_succ_le_zero 0) (λ a b c, b (le_of_succ_le_succ c)) n
 
-  attribute [simp]
-  lemma zero_sub_eq_zero : ∀ a : ℕ, 0 - a = 0
-  | 0     := rfl
-  | (a+1) := congr_arg pred (zero_sub_eq_zero a)
+  protected lemma lt_irrefl (n : ℕ) : ¬n < n :=
+  not_succ_le_self n
 
-  lemma zero_eq_zero_sub (a : ℕ) : 0 = 0 - a :=
-  eq.symm (zero_sub_eq_zero a)
+  protected lemma le_trans {n m k : ℕ} (h1 : n ≤ m) : m ≤ k → n ≤ k :=
+  le.rec h1 (λ p h2, le.step)
+
+  lemma pred_le : ∀ (n : ℕ), pred n ≤ n
+  | 0        := le.nat_refl 0
+  | (succ a) := le.step (le.nat_refl a)
 
   lemma sub_le (a b : ℕ) : a - b ≤ a :=
   nat.rec_on b (nat.le_refl (a - 0)) (λ b₁, nat.le_trans (pred_le (a - b₁)))
-
-  attribute [simp]
-  lemma sub_le_iff_true (a b : ℕ) : a - b ≤ a ↔ true :=
-  iff_true_intro (sub_le a b)
 
   lemma sub_lt : ∀ {a b : ℕ}, 0 < a → 0 < b → a - b < a
   | 0     b     h1 h2 := absurd h1 (nat.lt_irrefl 0)
@@ -348,24 +134,7 @@ namespace nat
       show a - b < succ a, from
       lt_succ_of_le (sub_le a b)
 
-  lemma sub_lt_succ (a b : ℕ) : a - b < succ a :=
-  lt_succ_of_le (sub_le a b)
+  protected lemma lt_of_lt_of_le {n m k : ℕ} : n < m → m ≤ k → n < k :=
+  nat.le_trans
 
-  attribute [simp]
-  lemma sub_lt_succ_iff_true (a b : ℕ) : a - b < succ a ↔ true :=
-  iff_true_intro (sub_lt_succ a b)
-
-  lemma le_add_right : ∀ (n k : ℕ), n ≤ n + k
-  | n 0     := nat.le_refl n
-  | n (k+1) := le_succ_of_le (le_add_right n k)
-
-  lemma le_add_left (n m : ℕ): n ≤ m + n :=
-  nat.add_comm n m ▸ le_add_right n m
-
-  def {u} repeat {α : Type u} (f : ℕ → α → α) : ℕ → α → α
-  | 0         a := a
-  | (succ n)  a := f n (repeat n a)
-
-  instance : inhabited ℕ :=
-  ⟨nat.zero⟩
 end nat
